investigations/cava2/Sha256Properties.v
@@ -1,0 +1,69 @@
+(****************************************************************************)
+(* Copyright 2021 The Project Oak Authors                                   *)
+(*                                                                          *)
+(* Licensed under the Apache License, Version 2.0 (the "License")           *)
+(* you may not use this file except in compliance with the License.         *)
+(* You may obtain a copy of the License at                                  *)
+(*                                                                          *)
+(*     http://www.apache.org/licenses/LICENSE-2.0                           *)
+(*                                                                          *)
+(* Unless required by applicable law or agreed to in writing, software      *)
+(* distributed under the License is distributed on an "AS IS" BASIS,        *)
+(* WITHOUT WARRANTIES OR CONDITIONS OF ANY KIND, either express or implied. *)
+(* See the License for the specific language governing permissions and      *)
+(* limitations under the License.                                           *)
+(****************************************************************************)
+
+Require Import Coq.Init.Byte.
+Require Import Coq.Lists.List.
+Require Import Coq.micromega.Lia.
+Require Import Coq.NArith.NArith.
+Require Import Cava.Types.
+Require Import Cava.Expr.
+Require Import Cava.Primitives.
+Require Import Cava.Semantics.
+Require Import Cava.Sha256.
+Require Import Cava.Util.List.
+Require Import Cava.Util.Tactics.
+Require HmacSpec.SHA256.
+Import ListNotations.
+
+(* TODO: move to a more general file *)
+Lemma step_vec_as_tuple_cons {t n} x0 (xs : list (denote_type t)) :
+  step (vec_as_tuple (t:=t) (n:=S n)) tt (x0 :: xs, tt)
+  = (tt, (x0, snd (step (vec_as_tuple (t:=t) (n:=n)) tt (xs, tt)))).
+Proof. reflexivity. Qed.
+Hint Rewrite @step_vec_as_tuple_cons using solve [eauto] : stepsimpl.
+Lemma step_vec_as_tuple_one {t} (x : denote_type t):
+  step (vec_as_tuple (t:=t) (n:=0)) tt ([x], tt) = (tt, x).
+Proof. reflexivity. Qed.
+Hint Rewrite @step_vec_as_tuple_one using solve [eauto] : stepsimpl.
+Ltac stepsimpl :=
+  repeat first [ progress
+                   cbn [fst snd step denote_type absorb_any
+                            split_absorbed_denotation combine_absorbed_denotation
+                            unary_semantics binary_semantics ]
+               | progress autorewrite with stepsimpl ].
+
+Lemma step_rotr n (x : denote_type sha_word) :
+  step (rotr n) tt (x,tt) = (tt, SHA256.ROTR (N.of_nat n) x).
+Proof.
+  cbv [rotr]. stepsimpl.
+  cbv [SHA256.ROTR SHA256.truncating_shiftl SHA256.w].
+  repeat (f_equal; try lia).
+Qed.
+Hint Rewrite @step_rotr using solve [eauto] : stepsimpl.
+
+Lemma step_sha256_compress
+      (H : denote_type sha_digest)
+      (k w : denote_type sha_word) (t i : nat) (msg : list byte) :
+  length H = 8 ->
+  k = nth t SHA256.K 0%N ->
+  w = nth t (SHA256.W msg i) 0%N ->
+  step sha256_compress tt (H,(k,(w,tt)))
+  = (tt, SHA256.sha256_compress msg i H t).
+Proof.
+  intros. subst; destruct_lists_by_length.
+  cbv [sha256_compress]. stepsimpl. reflexivity.
+Qed.
+Hint Rewrite @step_sha256_compress using solve [eauto] : stepsimpl.
